Dataflow/Syntax.v
@@ -115,20 +115,29 @@ Module Type SYNTAX
     | Ewhen e _ _ => typeof e
     end.
 
-  Definition memory_eq (mems: PS.t) (eq: equation) : PS.t :=
-    match eq with
-    | EqFby x _ _ _ => PS.add x mems
-    | _ => mems
-    end.
-
-  Definition memories (eqs: list equation) : PS.t :=
-    List.fold_left memory_eq eqs PS.empty.
-
   Definition var_defined (eq: equation) : ident :=
     match eq with
     | EqDef x _ _ => x
     | EqApp x _ _ _ _ => x
     | EqFby x _ _ _ => x
+    end.
+
+  Definition is_fby (eq: equation) : bool :=
+    match eq with
+    | EqFby _ _ _ _ => true
+    | _ => false
+    end.
+
+  Definition is_app (eq: equation) : bool :=
+    match eq with
+    | EqApp _ _ _ _ _ => true
+    | _ => false
+    end.
+
+  Definition is_def (eq: equation) : bool :=
+    match eq with
+    | EqDef _ _ _ => true
+    | _ => false
     end.
 
   Record node : Type :=
@@ -142,7 +151,7 @@ Module Type SYNTAX
         n_ingt0 : 0 < length n_in;
         n_defd  : Permutation (map var_defined n_eqs)
                               (map fst (n_vars ++ [n_out]));
-        n_vout  : ~PS.In (fst n_out) (memories n_eqs);
+        n_vout  : ~In (fst n_out) (map var_defined (filter is_fby n_eqs));
         n_decl  : Forall (VarsDeclared (n_in ++ n_vars ++ [n_out])) n_eqs;
         n_nodup : NoDupMembers (n_in ++ n_vars ++ [n_out]);
         n_good  : Forall NotReserved (n_in ++ n_vars ++ [n_out])
@@ -157,6 +166,27 @@ Module Type SYNTAX
   (* definition is needed in signature *)
   Definition find_node (f : ident) : global -> option node :=
     List.find (fun n=> ident_eqb n.(n_name) f).
+
+  (** Structural properties *)
+
+  Lemma is_filtered_eqs:
+    forall eqs,
+      Permutation
+        (filter is_def eqs ++ filter is_app eqs ++ filter is_fby eqs)
+        eqs.
+  Proof.
+    induction eqs as [|eq eqs]; auto.
+    destruct eq; simpl.
+    - now apply Permutation_cons.
+    - rewrite <-Permutation_cons_app.
+      apply Permutation_cons; reflexivity.
+      now symmetry.
+    - symmetry.
+      rewrite <-Permutation_app_assoc.
+      apply Permutation_cons_app.
+      rewrite Permutation_app_assoc.
+      now symmetry.
+  Qed.
 
 End SYNTAX.
 
